pull out definition to extract values from a list of store values

compiler/proofs/intLangExtraScript.sml
@@ -78,8 +78,11 @@ val all_vlabs_list_MAP = store_thm("all_vlabs_list_MAP",
   Induct >> rw[])
 val _ = export_rewrites["no_vlabs_list_MAP","all_vlabs_list_MAP"]
 
+val store_vs_def = Define`
+  store_vs s = MAP dest_Refv (FILTER is_Refv s)`
+
 val vlabs_csg_def = Define
-  `vlabs_csg csg = vlabs_list (MAP dest_Refv (FILTER is_Refv (SND(FST csg)))) ∪ vlabs_list (MAP THE (FILTER IS_SOME (SND csg)))`
+  `vlabs_csg csg = vlabs_list (store_vs (SND(FST csg))) ∪ vlabs_list (MAP THE (FILTER IS_SOME (SND csg)))`
 
 val Cevaluate_vlabs = store_thm("Cevaluate_vlabs",
   ``(∀s env exp res. Cevaluate s env exp res ⇒
@@ -187,7 +190,7 @@ val Cevaluate_vlabs = store_thm("Cevaluate_vlabs",
     Cases >> rw[] >>
     fs[el_check_def,EVERY_MEM] >>
     BasicProvers.EVERY_CASE_TAC >>
-    fsrw_tac[DNF_ss][SUBSET_DEF,vlabs_list_MAP,vlabs_csg_def] >> rw[] >>
+    fsrw_tac[DNF_ss][SUBSET_DEF,vlabs_list_MAP,vlabs_csg_def,store_vs_def] >> rw[] >>
     fs[MEM_MAP,PULL_EXISTS,MEM_FILTER] >> rw[] >>
     fs[vlabs_list_MAP] >> rw[] >>
     metis_tac[MEM_EL,dest_Refv_def,is_Refv_def])>>
@@ -200,7 +203,7 @@ val Cevaluate_vlabs = store_thm("Cevaluate_vlabs",
       Cases_on`op`>>Cases_on`v1`>>Cases_on`v2`>>fs[CevalPrim2s_def] >>
       TRY(Cases_on`l:lit`)>>TRY(Cases_on`l':lit`)>>fs[CevalPrim2s_def] >>
       pop_assum mp_tac >> rw[] >>
-      fs[vlabs_csg_def,FILTER_APPEND] >>
+      fs[vlabs_csg_def,store_vs_def,FILTER_APPEND] >>
       BasicProvers.EVERY_CASE_TAC >> fs[] >> rw[]) >>
     qmatch_assum_rename_tac`CevalPrim2p op v1 v2 = res`["res"] >>
     Cases_on`op`>>fs[CevalPrim2p_def]>>
@@ -218,15 +221,15 @@ val Cevaluate_vlabs = store_thm("Cevaluate_vlabs",
       Cases_on`v3`>>fs[]>>
       Cases_on`l`>>fs[]>>
       BasicProvers.EVERY_CASE_TAC>>fs[]>>rw[]>>
-      fsrw_tac[DNF_ss][vlabs_csg_def,SUBSET_DEF,vlabs_list_MAP,MEM_MAP,PULL_EXISTS,MEM_FILTER] >>
+      fsrw_tac[DNF_ss][vlabs_csg_def,store_vs_def,SUBSET_DEF,vlabs_list_MAP,MEM_MAP,PULL_EXISTS,MEM_FILTER] >>
       metis_tac[MEM_LUPDATE_E,is_Refv_def,dest_Refv_def] ) >>
-    fsrw_tac[DNF_ss][SUBSET_DEF,vlabs_list_MAP,vlabs_csg_def,MEM_MAP,PULL_EXISTS,MEM_FILTER] >>
+    fsrw_tac[DNF_ss][SUBSET_DEF,vlabs_list_MAP,vlabs_csg_def,store_vs_def,MEM_MAP,PULL_EXISTS,MEM_FILTER] >>
     metis_tac[MEM_LUPDATE_E,is_Refv_def,dest_Refv_def] ) >>
   strip_tac >- rw[] >>
   strip_tac >- ( srw_tac[DNF_ss][SUBSET_DEF] >> metis_tac[] ) >>
   strip_tac >- ( srw_tac[DNF_ss][SUBSET_DEF] >> metis_tac[] ) >>
   strip_tac >- (
-    srw_tac[DNF_ss][SUBSET_DEF,vlabs_csg_def,FILTER_APPEND,vlabs_list_APPEND] >>
+    srw_tac[DNF_ss][SUBSET_DEF,vlabs_csg_def,store_vs_def,FILTER_APPEND,vlabs_list_APPEND] >>
     fs[vlabs_list_MAP,MEM_MAP,MEM_FILTER,MEM_GENLIST] >> fs[]) >>
   strip_tac >- ( srw_tac[DNF_ss][SUBSET_DEF] >> metis_tac[] ) >>
   strip_tac >- ( srw_tac[DNF_ss][SUBSET_DEF] >> metis_tac[] ) >>
@@ -234,10 +237,10 @@ val Cevaluate_vlabs = store_thm("Cevaluate_vlabs",
   strip_tac >- ( srw_tac[DNF_ss][SUBSET_DEF] >> metis_tac[] ));
 
 val no_vlabs_csg_def = Define`no_vlabs_csg csg ⇔
-  no_vlabs_list (MAP dest_Refv (FILTER is_Refv (SND (FST csg)))) ∧
+  no_vlabs_list (store_vs (SND (FST csg))) ∧
   no_vlabs_list (MAP THE (FILTER IS_SOME (SND csg)))`
 val all_vlabs_csg_def = Define`all_vlabs_csg csg ⇔
-  all_vlabs_list (MAP dest_Refv (FILTER is_Refv (SND (FST csg)))) ∧
+  all_vlabs_list (store_vs (SND (FST csg))) ∧
   all_vlabs_list (MAP THE (FILTER IS_SOME (SND csg)))`
 
 val tac =
@@ -249,7 +252,7 @@ val tac =
   strip_tac >- simp[] >>
   strip_tac >- fsrw_tac[DNF_ss][EVERY_MEM,MEM_EL] >>
   strip_tac >- (
-    fsrw_tac[DNF_ss][EVERY_MEM,no_vlabs_csg_def,all_vlabs_csg_def,MEM_MAP,MEM_FILTER] >>
+    fsrw_tac[DNF_ss][EVERY_MEM,no_vlabs_csg_def,all_vlabs_csg_def,store_vs_def,MEM_MAP,MEM_FILTER] >>
     rw[MEM_EL,PULL_EXISTS] >>
     rpt (first_x_assum(qspec_then`n`mp_tac)) >>
     simp[] ) >>
@@ -270,7 +273,7 @@ val tac =
     first_x_assum match_mp_tac >>
     simp[EVERY_MAP,EVERY_GENLIST] >>
     fsrw_tac[DNF_ss][EVERY_MEM,MEM_EL] >>
-    fs[no_vlabs_csg_def,all_vlabs_csg_def] >>
+    fs[no_vlabs_csg_def,all_vlabs_csg_def,store_vs_def] >>
     metis_tac[no_labs_def,all_labs_def] ) >>
   strip_tac >- fsrw_tac[DNF_ss][EVERY_MEM,MEM_EL] >>
   strip_tac >- fsrw_tac[DNF_ss][EVERY_MEM,MEM_EL] >>
@@ -279,7 +282,7 @@ val tac =
     ntac 2 gen_tac >>
     reverse Cases >- (
       simp[] >> rw[] >>
-      fs[no_vlabs_csg_def,all_vlabs_csg_def,EVERY_MAP,EVERY_MEM,MEM_FILTER,MEM_LUPDATE,PULL_EXISTS] >>
+      fs[no_vlabs_csg_def,all_vlabs_csg_def,store_vs_def,EVERY_MAP,EVERY_MEM,MEM_FILTER,MEM_LUPDATE,PULL_EXISTS] >>
       Cases >> simp[] >> rw[] >> rw[] >>
       metis_tac[MEM_EL,optionTheory.IS_SOME_DEF,optionTheory.THE_DEF] ) >>
     ntac 4 gen_tac >>
@@ -288,14 +291,18 @@ val tac =
     TRY (
       pop_assum mp_tac >> BasicProvers.CASE_TAC>>fs[]>>
       BasicProvers.CASE_TAC>>rw[]>>
-      fs[no_vlabs_csg_def,all_vlabs_csg_def,EVERY_MAP,EVERY_MEM,MEM_FILTER] >>
+      fs[no_vlabs_csg_def,all_vlabs_csg_def,store_vs_def] >>
+      fs[EVERY_MAP,EVERY_MEM,MEM_FILTER] >>
       metis_tac[MEM_EL,is_Refv_def,dest_Refv_def] ) >>
     TRY (
-      fsrw_tac[DNF_ss][no_vlabs_csg_def,all_vlabs_csg_def,EVERY_MAP,EVERY_MEM,MEM_FILTER] >>
+      fsrw_tac[DNF_ss][no_vlabs_csg_def,all_vlabs_csg_def,store_vs_def] >>
+      fs[EVERY_MAP,EVERY_MEM,MEM_FILTER] >>
       NO_TAC ) >>
     BasicProvers.EVERY_CASE_TAC >>
     fsrw_tac[DNF_ss][EVERY_MEM,MEM_EL] >>
-    fsrw_tac[DNF_ss][no_vlabs_csg_def,all_vlabs_csg_def,EVERY_MEM,MEM_EL] >>
+    fsrw_tac[DNF_ss][no_vlabs_csg_def,all_vlabs_csg_def,store_vs_def] >>
+    fsrw_tac[DNF_ss][EVERY_MAP,EVERY_FILTER] >>
+    fs[EVERY_MEM] >>
     TRY(
       gen_tac >> strip_tac >>
       qmatch_assum_rename_tac`nn < LENGTH ll + 1`[] >>
@@ -313,7 +320,7 @@ val tac =
       Cases_on`op`>>Cases_on`v1`>>Cases_on`v2`>>fs[CevalPrim2s_def] >>
       TRY(Cases_on`l:lit`)>>TRY(Cases_on`l':lit`)>>fs[CevalPrim2s_def] >>
       pop_assum mp_tac >> rw[] >>
-      fs[no_vlabs_csg_def,all_vlabs_csg_def,FILTER_APPEND] >>
+      fs[no_vlabs_csg_def,all_vlabs_csg_def,store_vs_def,FILTER_APPEND] >>
       BasicProvers.EVERY_CASE_TAC >> fs[] >> rw[]) >>
     qmatch_assum_rename_tac`CevalPrim2p op v1 v2 = res`["res"] >>
     Cases_on`op`>>fs[CevalPrim2p_def]>>
@@ -331,17 +338,17 @@ val tac =
       Cases_on`v3`>>fs[]>>
       Cases_on`l`>>fs[]>>
       BasicProvers.EVERY_CASE_TAC>>fs[]>>rw[]>>
-      fsrw_tac[DNF_ss][no_vlabs_csg_def,all_vlabs_csg_def,SUBSET_DEF,no_vlabs_list_MAP,all_vlabs_list_MAP,MEM_MAP,PULL_EXISTS,MEM_FILTER,EVERY_MAP,EVERY_MEM] >>
+      fsrw_tac[DNF_ss][no_vlabs_csg_def,all_vlabs_csg_def,store_vs_def,SUBSET_DEF,no_vlabs_list_MAP,all_vlabs_list_MAP,MEM_MAP,PULL_EXISTS,MEM_FILTER,EVERY_MAP,EVERY_MEM] >>
       metis_tac[MEM_LUPDATE_E,is_Refv_def,dest_Refv_def] ) >>
     BasicProvers.EVERY_CASE_TAC >>
-    fsrw_tac[DNF_ss][SUBSET_DEF,no_vlabs_list_MAP,all_vlabs_list_MAP,no_vlabs_csg_def,all_vlabs_csg_def,MEM_MAP,PULL_EXISTS,MEM_FILTER,EVERY_MAP,EVERY_FILTER,EVERY_MEM] >>
+    fsrw_tac[DNF_ss][SUBSET_DEF,no_vlabs_list_MAP,all_vlabs_list_MAP,no_vlabs_csg_def,all_vlabs_csg_def,store_vs_def,MEM_MAP,PULL_EXISTS,MEM_FILTER,EVERY_MAP,EVERY_FILTER,EVERY_MEM] >>
     metis_tac[MEM_LUPDATE_E,is_Refv_def,dest_Refv_def] ) >>
   strip_tac >- fsrw_tac[DNF_ss][EVERY_MEM,MEM_EL] >>
   strip_tac >- (
     ntac 6 gen_tac >>
     Cases >> fsrw_tac[DNF_ss][EVERY_MEM,MEM_EL] ) >>
   strip_tac >- fsrw_tac[DNF_ss][EVERY_MEM,MEM_EL] >>
-  strip_tac >- fsrw_tac[DNF_ss][no_vlabs_csg_def,all_vlabs_csg_def,EVERY_MAP,EVERY_FILTER,EVERY_GENLIST] >>
+  strip_tac >- fsrw_tac[DNF_ss][no_vlabs_csg_def,all_vlabs_csg_def,store_vs_def,EVERY_MAP,EVERY_FILTER,EVERY_GENLIST] >>
   strip_tac >- fsrw_tac[DNF_ss][EVERY_MEM,MEM_EL] >>
   strip_tac >- ( rw[] >> fsrw_tac[DNF_ss][EVERY_MEM,MEM_EL] ) >>
   strip_tac >- fsrw_tac[DNF_ss][EVERY_MEM,MEM_EL] >>
